Bloom filter protocol in progress

examples/crypto/bloom-format.fst
@@ -1,11 +1,13 @@
 module Format
 
 open FStar.Seq
+open FStar.SeqProperties
 
 type uint = i:int{0 <= i}
 type pint = i:int{1 <= i}
 
-type msg (i:pint) = m:seq byte{length m = i}
+type message = seq byte
+type msg (i:pint) = m:message{length m = i}
 
 val max_int : i:pint -> Tot uint
 let rec max_int i =
@@ -29,3 +31,32 @@ let uint32_to_bytes = ulint_to_bytes 4
 val bytes_to_uint16: msg 2 -> Tot uint16
 let bytes_to_uint16 = bytes_to_ulint 2
 let bytes_to_uint32 = bytes_to_ulint 4
+
+let tag0 = create 1 0uy
+
+val signal_size: int
+let signal_size = 7 (* Bytes *)
+
+val signal : uint32 -> uint16 -> Tot (msg signal_size)
+let signal s c =
+  let s_b = uint32_to_bytes s in
+  let c_b = uint16_to_bytes c in
+  append tag0 (append s_b c_b)
+
+val signal_split : m:msg signal_size -> Tot (x:option (uint32 * uint16)
+    { is_Some x ==> m = signal (fst (Some.v x)) (snd (Some.v x))})
+let signal_split m =
+  let (t, sc) = split_eq m 1 in
+  if t = tag0 then
+    let (s_b, c_b) = split_eq sc 4 in
+    let (s, c) = (bytes_to_ulint 4 s_b, bytes_to_ulint 2 c_b) in
+    Some (s, c)
+  else
+    None
+
+val signal_components_corr:
+  s0:uint32 -> c0:uint16 -> s1:uint32 -> c1:uint16 ->
+  Lemma (requires (Seq.Eq (signal s0 c0) (signal s1 c1)))
+        (ensures  (s0 = s1 /\ c0 = c1))
+        [SMTPat (signal s0 c0); SMTPat (signal s1 c1)]
+let signal_components_corr s0 c0 s1 c1 = ()
